removed implicit args from term triples and graph, removes redundant condition over rdf_graphs and fix proofs. + some other minor changes

src/Rdf.v
@@ -8,198 +8,133 @@ From RDF Require Import Triple.
 Section Rdf.
   Axiom todo_rdf: forall t, t.
 
-  Record rdf_graph {I B L : Type}:= mkRdfGraph {
-                                       graph : seq triple
-                                     ; subject_in_IB : all (fun t => @is_in_ib I B L (subject t)) graph
-                                     ; predicate_in_I : all (fun t => @is_in_i I B L (predicate t)) graph
-                                     ; object_in_IBL : all (fun t => @is_in_ibl I B L (object t)) graph
+  Record rdf_graph (I B L : Type):= mkRdfGraph {
+                                       graph : seq (triple I B L)
                                      }.
-
-  Lemma forget_hd {T : Type} {t : T} {st : seq T} {p: T -> bool} (pall: all p (t::st)) : all p st.
-  Proof. revert pall=> /=. by move /andP=> [_ ->]. Qed.
-
-  Lemma graph_inj {I B L : Type}: forall (g1 g2: @rdf_graph I B L),
-      graph g1 = graph g2 ->
-      g1 = g2.
-  Proof.
-    move=> [g1 sib1 pi1 oibl1] [g2 sib2 pi2 oibl2] /= geq. 
-    by subst; f_equal; apply eq_irrelevance.
-  Qed.
-
 
   Section PolyRdf.
     Variables I B L : Type.
 
-    Definition empty_sib : all (fun t => @is_in_ib I B L (subject t)) [::]. Proof. by []. Qed.
-    Definition empty_pii :  all (fun t => @is_in_i I B L (predicate t)) [::]. Proof. by []. Qed.
-    Definition empty_oibl : all (fun t => @is_in_ibl I B L (object t)) [::]. Proof. by []. Qed.
+    Definition empty_rdf_graph : rdf_graph I B L:= mkRdfGraph [::].
 
-    Definition empty_rdf_graph : @rdf_graph I B L:= mkRdfGraph empty_sib empty_pii empty_oibl.
+    Definition is_ground(g : rdf_graph I B L) : bool :=
+      all (@is_ground_triple I B L) (graph g).
 
-    Definition is_ground(g : @rdf_graph I B L) : bool :=
-      foldr andb true (map (@is_ground_triple I B L) (graph g)).
-
-    Definition merge_rdf_graph (g h : @rdf_graph I B L) : @rdf_graph I B L :=
+    (* assumes shared identifier scope *)
+    Definition merge_rdf_graph (g h : rdf_graph I B L) : rdf_graph I B L :=
       todo_rdf _.
 
-    Definition merge_seq_rdf_graph (gs : seq (@rdf_graph I B L)) : @rdf_graph I B L :=
+    Definition merge_seq_rdf_graph (gs : seq (rdf_graph I B L)) : rdf_graph I B L :=
       foldr merge_rdf_graph empty_rdf_graph gs.
-    
-    Definition add_sib (ts : seq triple) (pall : all (fun t => is_in_ib (subject t)) ts) (t : triple) : all (fun t => @is_in_ib I B L (subject t)) (t::ts).
-    Proof. elim (t::ts) => [//| a l ihl] /=.
-           - apply /andP ; split. by case a=> /= _ _ _ -> _ _. by apply ihl.
-    Qed.
 
-    Definition add_i (ts : seq triple) (pall : all (fun t => is_in_i (predicate t)) ts) (t : triple) : all (fun t => @is_in_i I B L (predicate t)) (t::ts).
-    Proof. elim (t::ts) => [//| a l ihl] /=.
-           - apply /andP ; split. by case a=> /= _ _ _ _ -> _. by apply ihl.
-    Qed.
-
-    Definition add_ibl (ts : seq triple) (pall : all (fun t => is_in_ibl (object t)) ts) (t : triple) : all (fun t => @is_in_ibl I B L (object t)) (t::ts).
-    Proof. elim (t::ts) => [//| a l ihl] /=.
-           - apply /andP ; split. by case a=> /= _ _ _ _ _ ->. by apply ihl.
-    Qed.
-
-    Definition add_triple (sg : option (@rdf_graph I B L)) (t : (@triple I B L)) : option (@rdf_graph I B L).
+    Definition add_triple (sg : option (rdf_graph I B L)) (t : (triple I B L)) : option (rdf_graph I B L).
     Proof. destruct sg as [g |].
            - destruct g as [g' sib ip ibl].
              exact (Some {|
                         graph := t :: g' ;
-                        subject_in_IB := (@add_sib g' sib t) ;
-                        predicate_in_I := (@add_i g' ip t) ;
-                        object_in_IBL := (@add_ibl g' ibl t)
                       |}).
            - exact None.
     Defined.
 
-    Definition relabeling_seq_triple (u' : Type) (μ : B -> u') (g : seq (@triple I B L)) : seq (@triple I u' L) :=
+    Definition relabeling_seq_triple (B' : Type) (μ : B -> B') (g : seq (triple I B L)) : seq (triple I B' L) :=
       map (relabeling_triple μ) g.
 
     Section Relabeling_seq_triple.
       Variable B' : Type.
 
-      Lemma relabeling_seq_triple_comp_P (g1 g2 : seq triple) (eqb : g1 = g2) (μ : B -> B') :
+      Lemma relabeling_seq_triple_comp_P (g1 g2 : seq (triple I B L)) (eqb : g1 = g2) (μ : B -> B') :
         relabeling_seq_triple μ g1 = relabeling_seq_triple μ g2.
       Proof. by rewrite eqb. Qed.
 
-      Lemma relabeling_seq_triple_comp (μ1 μ2 : B -> B) (g : seq triple) : @relabeling_seq_triple B μ1 (relabeling_seq_triple μ2 g) = (@relabeling_seq_triple B μ1 \o (relabeling_seq_triple μ2)) g.
+      Lemma relabeling_seq_triple_comp (μ1 μ2 : B -> B) (g : seq (triple I B L)) : relabeling_seq_triple μ1 (relabeling_seq_triple μ2 g) = (relabeling_seq_triple μ1 \o (relabeling_seq_triple μ2)) g.
       Proof. by []. Qed.
 
-      Lemma relabeling_seq_triple_preserves_subject_in_IB (g : seq triple) (μ : B -> B') :
-        all (fun t => @is_in_ib I B L (subject t)) g ->
-        all (fun t => @is_in_ib I B' L (subject t)) (relabeling_seq_triple μ g).
-      Proof. elim g => [//| a l ihl] /andP [sibh sibt]. apply /andP; split.
-             by apply relabeling_triple_preserves_is_in_ib; apply sibh.
-             by apply ihl; apply sibt.
-      Qed.
-
-      Lemma relabeling_seq_triple_preserves_predicate_in_I (g : seq triple) (μ : B -> B') :
-        all (fun t => is_in_i (predicate t)) g ->
-        all (fun t => is_in_i (predicate t)) (relabeling_seq_triple μ g).
-      Proof. elim g => [//| a l ihl] /andP [pinh pin]; apply /andP; split.
-             by apply relabeling_triple_preserves_is_in_i; apply pinh.
-             by apply ihl; apply pin.
-      Qed.
-
-      Lemma relabeling_seq_triple_preserves_object_in_IBL (g : seq triple) (μ : B -> B') :
-        all (fun t => is_in_ibl (object t)) g ->
-        all (fun t => is_in_ibl (object t)) (relabeling_seq_triple μ g).
-      Proof. elim g => [//| a l ihl] /andP [oinh oint]; apply /andP; split.
-             by apply relabeling_triple_preserves_is_in_ibl ; apply oinh.
-             by apply ihl; apply oint.
-      Qed.
-
-      Lemma relabeling_seq_triple_ext (μ1 μ2 : B -> B') : μ1 =1 μ2 -> forall g : seq (@triple I B L), relabeling_seq_triple μ1 g = relabeling_seq_triple μ2 g.
+      Lemma relabeling_seq_triple_ext (μ1 μ2 : B -> B') : μ1 =1 μ2 -> forall g : seq (triple I B L), relabeling_seq_triple μ1 g = relabeling_seq_triple μ2 g.
       Proof. move => μpqeq. elim=> [//|h t IHt] /=. rewrite IHt. f_equal. by apply relabeling_triple_ext . Qed.
     End Relabeling_seq_triple.
 
-    Lemma relabeling_seq_triple_id (g : seq triple) : @relabeling_seq_triple B id g = g.
+    Lemma relabeling_seq_triple_id (g : seq (triple I B L)) : relabeling_seq_triple id g = g.
     Proof. elim g => [//| a l ihl] /=. by rewrite relabeling_triple_id ihl.
     Qed.
 
-    Lemma relabeling_seq_triple_comp_simpl (g : seq triple) (μ12 μ23 : B -> B) :
-      relabeling_seq_triple (μ23 \o μ12) g = (@relabeling_seq_triple B μ23 \o (relabeling_seq_triple μ12)) g.
+    Lemma relabeling_seq_triple_comp_simpl (g : seq (triple _ _ _)) (μ12 μ23 : B -> B) :
+      relabeling_seq_triple (μ23 \o μ12) g = relabeling_seq_triple μ23 (relabeling_seq_triple μ12 g).
     Proof. elim g => [//|h t iht] /=. by rewrite relabeling_triple_comp; f_equal; apply iht.
     Qed.
 
+    Definition relabeling (B' : Type) (μ : B -> B') (g : rdf_graph I B L): rdf_graph I B' L:=
+      mkRdfGraph (relabeling_seq_triple μ (graph g)).
 
-    Definition relabeling (u' : Type) (μ : B -> u') (g : rdf_graph): rdf_graph :=
-      let (g',siib,pii,oiibl) := g in
-      {|
-        graph := relabeling_seq_triple μ g';
-        subject_in_IB :=  relabeling_seq_triple_preserves_subject_in_IB μ siib;
-        predicate_in_I := relabeling_seq_triple_preserves_predicate_in_I μ pii;
-        object_in_IBL := relabeling_seq_triple_preserves_object_in_IBL μ oiibl
-      |}.
-
-    Lemma relabeling_comp (g : rdf_graph) (μ12 μ23: B -> B) :
+    Lemma relabeling_comp (g : rdf_graph I B L) (μ12 μ23: B -> B) :
       (relabeling μ23 \o (relabeling μ12)) g = relabeling (μ23 \o μ12) g.
-    Proof. apply graph_inj; case g => g' /= _ _ _; by rewrite relabeling_seq_triple_comp_simpl.
+    Proof. by case g => g'; rewrite /relabeling relabeling_seq_triple_comp_simpl //=.
     Qed.
 
 
     Section Relabeling_graph.
       Variable B' : Type.
 
-      Lemma relabeling_id (g : rdf_graph) : relabeling id g = g.
-      Proof. apply graph_inj. case g => g' /= _ _ _. by rewrite relabeling_seq_triple_id.
+      Lemma relabeling_id (g : rdf_graph I B L) : relabeling id g = g.
+      Proof. case g => g' /=. by rewrite /relabeling relabeling_seq_triple_id.
       Qed.
 
       Lemma relabeling_ext  (μ1 μ2 : B -> B') :  μ1 =1 μ2 -> forall g, relabeling μ1 g = relabeling μ2 g.
-      Proof. move=> μpweq g. apply graph_inj. case g=> g' /= _ _ _. by apply relabeling_seq_triple_ext. Qed.
+      Proof. move=> μpweq g. by case g=> g'; rewrite /relabeling (relabeling_seq_triple_ext μpweq). Qed.
 
     End Relabeling_graph.
 
-    Lemma relabeling_comp_simpl (μ1 μ2 : B -> B) (g : rdf_graph) : relabeling μ1 (relabeling μ2 g) = relabeling (μ1 \o μ2) g.
+    Lemma relabeling_comp_simpl (μ1 μ2 : B -> B) (g : rdf_graph I B L) : relabeling μ1 (relabeling μ2 g) = relabeling (μ1 \o μ2) g.
     Proof. by rewrite -relabeling_comp. Qed.
 
   End PolyRdf.
   Section EqRdf.
     Variables I B L : eqType.
 
-    Definition eqb_rdf (g1 g2 : @rdf_graph I B L) : bool :=
+    Definition eqb_rdf (g1 g2 : rdf_graph I B L) : bool :=
       (graph g1) == (graph g2).
-    Lemma eqb_rdf_refl (g : rdf_graph) : eqb_rdf g g.
+
+    Lemma eqb_rdf_refl (g : rdf_graph I B L) : eqb_rdf g g.
     Proof. by rewrite /eqb_rdf. Qed.
 
-    Lemma eqb_rdf_symm (g1 g2 : rdf_graph) : eqb_rdf g1 g2 = eqb_rdf g2 g1.
+    Lemma eqb_rdf_symm (g1 g2 : rdf_graph I B L) : eqb_rdf g1 g2 = eqb_rdf g2 g1.
     Proof. by rewrite /eqb_rdf. Qed.
 
     Definition rdf_eqP : Equality.axiom eqb_rdf.
     Proof. rewrite /Equality.axiom => x y.
-           apply: (iffP idP) => //= [| ->];
-                               case: x y=> [g1 sib1 pi1 oibl1] [g2 sib2 pi2 oibl2]. rewrite /eqb_rdf => /eqP /= geq. subst. by apply graph_inj. by apply eqb_rdf_refl.
+           apply: (iffP idP) => //= [| ->]; case: x y=> [g1] [g2].
+           by rewrite /eqb_rdf => /eqP /= ->.
+           by apply eqb_rdf_refl.
     Qed.
 
-    Canonical rdf_eqType := EqType rdf_graph (EqMixin rdf_eqP).
+    Canonical rdf_eqType := EqType (rdf_graph I B L) (EqMixin rdf_eqP).
 
-    Definition terms (g : @rdf_graph I B L) : seq term :=
+    Definition terms (g : rdf_graph I B L) : seq (term _ _ _) :=
       flatten (map (fun t => terms_triple t) (graph g)).
 
-    Definition bnodes (g : @rdf_graph I B L) : seq term :=
+    Definition bnodes (g : rdf_graph I B L) : seq (term _ _ _) :=
       filter (fun t => is_bnode t) (terms g).
 
     Lemma bijective_eqb_rdf mu nu g1 g2 : cancel mu nu -> eqb_rdf g1 (relabeling mu g2) ->  eqb_rdf g2 (relabeling nu g1).
     Proof.
-      move=> cancel_mu_nu. rewrite /eqb_rdf => /eqP /graph_inj ->.
-      rewrite relabeling_comp_simpl.
-      have /relabeling_ext-> : nu \o mu =1 id by [].
-      rewrite relabeling_id; exact: eqb_rdf_refl.
+      move=> cancel_mu_nu. rewrite /eqb_rdf => /eqP /= ->.
+      rewrite -relabeling_seq_triple_comp_simpl. 
+      have /relabeling_seq_triple_ext-> : nu \o mu =1 id by [].
+      rewrite relabeling_seq_triple_id; exact: eqb_rdf_refl.
     Qed.
 
-    Definition is_iso (g1 g2 : @rdf_graph I B L) (μ : B -> B) :=
+    Definition is_iso (g1 g2 : rdf_graph I B L) (μ : B -> B) :=
       (bijective μ) /\ eqb_rdf g1 (relabeling μ g2).
 
-    Definition iso (g1 g2 : rdf_graph):= exists (μ : B -> B),
+    Definition iso (g1 g2 : rdf_graph I B L) := exists (μ : B -> B),
         is_iso g1 g2 μ.
 
-    Lemma iso_refl (g : rdf_graph) : iso g g.
+    Lemma iso_refl (g : rdf_graph I B L) : iso g g.
     Proof. rewrite /iso /is_iso; exists id; split.
            exists id => //.
            by rewrite relabeling_id eqb_rdf_refl.
     Qed.
 
-    Lemma iso_symm (g1 g2 : rdf_graph) :
+    Lemma iso_symm (g1 g2 : rdf_graph I B L) :
       iso g1 g2 <-> iso g2 g1.
     Proof.
       rewrite /iso /is_iso.
@@ -207,36 +142,32 @@ Section Rdf.
                                                          (exists nu; split; [exact: bij_can_bij h1 | exact: bijective_eqb_rdf heqb_rdf]).
     Qed.
 
-    Lemma iso_trans (g1 g2 g3: rdf_graph) : iso g1 g2 -> iso g2 g3 -> iso g1 g3.
-    Proof. rewrite /iso/is_iso/eqb_rdf => [[μ1 [bij1/eqP/graph_inj eqb1]] [μ2 [bij2/eqP/graph_inj eqb2]]].
+    Lemma iso_trans (g1 g2 g3: rdf_graph I B L) : iso g1 g2 -> iso g2 g3 -> iso g1 g3.
+    Proof. rewrite /iso/is_iso/eqb_rdf/relabeling => [[μ1 [bij1/eqP eqb1]] [μ2 [bij2/eqP eqb2]]].
            exists (μ1 \o μ2). split.
-           rewrite /=. apply bij_comp. apply bij1. apply bij2.
-           rewrite -relabeling_comp /= -eqb2 -eqb1. by apply eqb_rdf_refl.
+           by apply bij_comp.
+           by rewrite eqb1 eqb2 relabeling_seq_triple_comp_simpl. 
     Qed.
 
-    Definition isocanonical_mapping (M : rdf_graph -> rdf_graph) :=
-      forall (g : rdf_graph),
-        iso (M g) g /\ forall (h : rdf_graph), iso (M g) (M h) <-> iso g h.
+    Definition isocanonical_mapping (M : rdf_graph I B L -> rdf_graph I B L) :=
+      forall (g : rdf_graph I B L),
+        iso (M g) g /\ forall (h : rdf_graph I B L), iso (M g) (M h) <-> iso g h.
 
   End EqRdf.
 
   Section CountRdf.
     Variables I B L : countType.
 
-    Definition code_rdf (g : rdf_graph) :=
-      let (g',_,_,_) := g in
+    Definition code_rdf (g : rdf_graph I B L) :=
+      let (g') := g in
       GenTree.Node 0 (map (@code_triple I B L) g').
 
-    Definition decode_rdf (x : GenTree.tree nat) : option (@rdf_graph I B L).
+    Definition decode_rdf (x : GenTree.tree nat) : option (rdf_graph I B L).
     Proof. destruct x.
            - exact None.
            - destruct n as [| n'].
              + induction l as [| t ts IHts].
-               * exact (Some (mkRdfGraph
-                                (all_nil (fun t => is_in_ib (subject t)))
-                                (all_nil (fun t => is_in_i (predicate t)))
-                                (all_nil (fun t => is_in_ibl (object t)))
-                       )).
+               * exact (Some (mkRdfGraph [::])).
                * destruct (@decode_triple I B L t) as [t'|].
                  -- apply (@add_triple I B L IHts t').
                  -- exact None.
@@ -244,24 +175,20 @@ Section Rdf.
     Defined.
 
     Lemma cancel_rdf_encode : pcancel code_rdf decode_rdf.
-    Proof. case => g sib ii ibl. rewrite /code_rdf /decode_rdf.
+    Proof. case => g. rewrite /code_rdf /decode_rdf.
            induction g as [| t ts IHts].
-           - rewrite /=. f_equal. by apply graph_inj.
-           - rewrite /=.
-             have cant : (@decode_triple I B L (code_triple t)) = Some t. apply cancel_triple_encode.
-             rewrite cant. rewrite IHts.
-           - apply (forget_hd sib). apply (forget_hd ii). apply (forget_hd ibl).
-             move=> sib' ii' ibl'. rewrite /add_triple /=. f_equal. apply graph_inj. by rewrite /eqb_rdf.
+           - by [].
+           - by rewrite /= cancel_triple_encode IHts. 
     Qed.
 
     Definition rdf_canChoiceMixin := PcanChoiceMixin cancel_rdf_encode.
     Definition rdf_canCountMixin := PcanCountMixin cancel_rdf_encode.
 
-    Canonical rdf_choiceType := Eval hnf in ChoiceType rdf_graph rdf_canChoiceMixin.
-    Canonical rdf_countType := Eval hnf in CountType rdf_graph rdf_canCountMixin.
+    Canonical rdf_choiceType := Eval hnf in ChoiceType (rdf_graph I B L) rdf_canChoiceMixin.
+    Canonical rdf_countType := Eval hnf in CountType (rdf_graph I B L) rdf_canCountMixin.
 
     Definition rdf_canPOrderMixin := PcanPOrderMixin (@pickleK rdf_countType).
-    Canonical rdf_POrderType := Eval hnf in POrderType tt rdf_graph rdf_canPOrderMixin.
+    Canonical rdf_POrderType := Eval hnf in POrderType tt (rdf_graph I B L) rdf_canPOrderMixin.
 
   End CountRdf.
 End Rdf.
