src/Term.v
@@ -9,68 +9,68 @@ Section Term.
   (* literals should be of Datatype type, is not important for the moment*)
   Open Scope order_scope.
 
-  Inductive term {I B L : Type} : Type :=
+  Inductive term (I B L : Type) : Type :=
   | Iri (id: I)
   | Lit (l : L)
   | Bnode (name : B).
 
-  Definition is_lit (t u v : Type) (t : @term t u v) : bool :=
+  Definition is_lit (t u v : Type) (t : term t u v) : bool :=
     (match t with
      | Lit _ => true
      | _ => false
      end).
 
-  Definition is_iri (t u v : Type) (t : @term t u v) : bool :=
+  Definition is_iri (t u v : Type) (t : term t u v) : bool :=
     (match t with
      | Iri _ => true
      | _ => false
      end).
 
-  Definition is_bnode (t u v : Type) (t : @term t u v) : bool :=
+  Definition is_bnode (t u v : Type) (t : term t u v) : bool :=
     (match t with
      | Bnode _ => true
      | _ => false
      end).
 
-  Definition is_in_ib (t u v : Type) (t : @term t u v) : bool :=
+  Definition is_in_ib (t u v : Type) (t : term t u v) : bool :=
     is_iri t || is_bnode t.
 
-  Definition is_in_i (t u v : Type) (t : @term t u v) : bool :=
+  Definition is_in_i (t u v : Type) (t : term t u v) : bool :=
     is_iri t.
 
-  Definition is_in_ibl (t u v : Type) (t : @term t u v) : bool :=
+  Definition is_in_ibl (t u v : Type) (t : term t u v) : bool :=
     is_iri t || is_bnode t || is_lit t.
 
 
   Section Poly.
     Variables I B L : Type.
 
-    Definition relabeling_term (B' : Type) (μ : B -> B') (trm : (@term I B L)) : @term I B' L :=
+    Definition relabeling_term (B' : Type) (μ : B -> B') (trm : (term I B L)) : term I B' L :=
       match trm with
-      | Bnode name => Bnode (μ name)
-      | Iri i => Iri i
-      | Lit l => Lit l
+      | Bnode name => Bnode I L (μ name)
+      | Iri i => Iri B' L i
+      | Lit l => Lit I B' l
       end.
 
-    Lemma relabeling_term_id (t: term) : @relabeling_term B id t = t.
+    Lemma relabeling_term_id (t: term I B L) : relabeling_term id t = t.
     Proof. by case t. Qed.
 
-    Lemma relabeling_term_comp (T : Type) (t: term) (μ1 μ2 : B -> B) : relabeling_term (μ2 \o μ1) t = (@relabeling_term B μ2 \o (relabeling_term μ1)) t.
+    Lemma relabeling_term_comp (T : Type) (t: term I B L) (μ1 μ2 : B -> B) : relabeling_term (μ2 \o μ1) t = (relabeling_term μ2 \o (relabeling_term μ1)) t.
     Proof. by case t. Qed.
 
     Section Relabeling_term.
       Variable B' : Type.
 
-      Lemma relabeling_term_preserves_is_in_ib (μ : B -> B') (t : @term I B L) : is_in_ib t <-> is_in_ib (relabeling_term μ t).
+      Lemma relabeling_term_preserves_is_in_ib (μ : B -> B') (t : term I B L) : is_in_ib t <-> is_in_ib (relabeling_term μ t).
+    Proof. by case t. Qed.
+
+      Lemma relabeling_term_preserves_is_in_i (μ : B -> B') (t : term I B L) : is_in_i t <-> is_in_i (relabeling_term μ t).
       Proof. by case t. Qed.
 
-      Lemma relabeling_term_preserves_is_in_i (μ : B -> B') (t : @term I B L) : is_in_i t <-> is_in_i (relabeling_term μ t).
+      Lemma relabeling_term_preserves_is_in_ibl (μ : B -> B') (t : term I B L) : is_in_ibl t <-> is_in_ibl (relabeling_term μ t).
       Proof. by case t. Qed.
 
-      Lemma relabeling_term_preserves_is_in_ibl (μ : B -> B') (t : @term I B L) : is_in_ibl t <-> is_in_ibl (relabeling_term μ t).
-      Proof. by case t. Qed.
-
-      Lemma relabeling_term_ext (μ1 μ2 : B -> B') : μ1 =1 μ2 -> forall t : @term I B L, relabeling_term μ1 t = relabeling_term μ2 t.
+      Lemma relabeling_term_ext (μ1 μ2 : B -> B') : μ1 =1 μ2 -> forall t : term I B L, relabeling_term μ1 t = relabeling_term μ2 t.
       Proof. move => μpweq [//| // | b] /=. by rewrite μpweq. Qed.
 
     End Relabeling_term.
@@ -79,7 +79,7 @@ Section Term.
   Section EqTerm.
     Variables I B L : eqType.
 
-    Definition eqb_term (t1 t2 : @term I B L) : bool :=
+    Definition eqb_term (t1 t2 : term I B L) : bool :=
       match t1, t2 with
       | Iri i1, Iri i2 => i1 == i2
       | Bnode b1, Bnode b2 => b1 == b2
@@ -94,24 +94,24 @@ Section Term.
       by case: x y=> [i1|l1|b1] [i2|l2|b2] // => /eqP ->.
     Qed.
 
-    Canonical term_eqType := EqType term (EqMixin term_eqP).
+    Canonical term_eqType := EqType (term I B L) (EqMixin term_eqP).
 
   End EqTerm.
   Section CountTerm.
     Variable I B L: countType.
 
-    Definition code_term (x : (@term I B L)) :=
+    Definition code_term (x : (term I B L)) :=
       match x with
       | Iri id => GenTree.Node 0 (GenTree.Leaf (pickle id) :: nil)
       | Lit l => GenTree.Node 1 (GenTree.Leaf (pickle l) :: nil)
       | Bnode name => GenTree.Node 2 (GenTree.Leaf (pickle name) :: nil)
       end.
 
-    Definition decode_term (x : GenTree.tree nat) : option (@term I B L) :=
+    Definition decode_term (x : GenTree.tree nat) : option (term I B L) :=
       match x with
-      | GenTree.Node 0 (GenTree.Leaf id :: nil) => omap Iri (unpickle id)
-      | GenTree.Node 1 (GenTree.Leaf l :: nil) =>  omap Lit (unpickle l)
-      | GenTree.Node 2 (GenTree.Leaf name :: nil) => omap Bnode (unpickle name)
+      | GenTree.Node 0 (GenTree.Leaf i :: nil) => omap (@Iri I B L) (unpickle i)
+      | GenTree.Node 1 (GenTree.Leaf l :: nil) =>  omap (@Lit I B L) (unpickle l)
+      | GenTree.Node 2 (GenTree.Leaf name :: nil) => omap (@Bnode I B L) (unpickle name)
       | _ => None
       end.
 
@@ -121,11 +121,11 @@ Section Term.
     Definition term_canChoiceMixin := PcanChoiceMixin cancel_code_decode.
     Definition term_canCountMixin := PcanCountMixin cancel_code_decode.
 
-    Canonical term_choiceType := Eval hnf in ChoiceType term term_canChoiceMixin.
-    Canonical term_countType := Eval hnf in CountType term term_canCountMixin.
+    Canonical term_choiceType := Eval hnf in ChoiceType (term I B L) term_canChoiceMixin.
+    Canonical term_countType := Eval hnf in CountType (term I B L) term_canCountMixin.
 
     Definition term_canPOrderMixin := PcanPOrderMixin (@pickleK term_countType).
-    Canonical term_POrderType := Eval hnf in POrderType tt term term_canPOrderMixin.
+    Canonical term_POrderType := Eval hnf in POrderType tt term_countType term_canPOrderMixin.
 
   End CountTerm.
 End Term.
