src/Triple.v
@@ -6,15 +6,15 @@ From RDF Require Import Term.
 
 Section Triple.
 
-  Record triple {I B L : Type} := mkTriple { subject : @term I B L
-                                           ; predicate : @term I B L
-                                           ; object: @term I B L
+  Record triple (I B L : Type) := mkTriple { subject : (term I B L)
+                                           ; predicate : (term I B L)
+                                           ; object: (term I B L)
                                            ; subject_in_IB: is_in_ib subject
                                            ; predicate_in_I: is_in_i predicate
                                            ; object_in_IBL: is_in_ibl object
                                    }.
 
-  Lemma triple_inj {I B L: Type}: forall (t1 t2: @triple I B L),
+  Lemma triple_inj {I B L: Type}: forall (t1 t2: triple I B L),
       subject t1 = subject t2 ->
       predicate t1 = predicate t2 ->
       object t1 = object t2 ->
@@ -27,41 +27,41 @@ Section Triple.
   Section PolyTriple.
     Variables I B L : Type.
 
-    Definition is_ground_triple (t : @triple I B L) : bool:=
+    Definition is_ground_triple (t : triple I B L) : bool:=
       let (s,p,o,_,_,_) := t in
       ~~ (is_bnode s || is_bnode p || is_bnode o).
 
-    Definition relabeling_triple (u' : Type) (μ : B -> u') (t : @triple I B L) : @triple I u' L :=
+    Definition relabeling_triple (B' : Type) (μ : B -> B') (t : triple I B L) : triple I B' L :=
       let (s,p,o,sin,pin,oin) := t in
       mkTriple ((iffLR (relabeling_term_preserves_is_in_ib μ s)) sin)
                ((iffLR (relabeling_term_preserves_is_in_i μ p)) pin)
                ((iffLR (relabeling_term_preserves_is_in_ibl μ o)) oin).
 
-    Lemma relabeling_triple_id (t : triple) : @relabeling_triple B id t = t.
+    Lemma relabeling_triple_id (t : triple I B L) : relabeling_triple id t = t.
     Proof.
       case t => [s p o sin pin oin] /=. apply triple_inj => /=; by apply relabeling_term_id. Qed.
 
-    Lemma relabeling_triple_comp (μ1 μ2 : B -> B) (t : triple) : relabeling_triple (μ2 \o μ1) t = (@relabeling_triple B μ2 \o (relabeling_triple μ1)) t.
+    Lemma relabeling_triple_comp (μ1 μ2 : B -> B) (t : (triple I B L)) : relabeling_triple (μ2 \o μ1) t = (relabeling_triple μ2 \o (relabeling_triple μ1)) t.
     Proof. case t=> [s p o sin pin oin] /=. apply triple_inj=> /=; by rewrite relabeling_term_comp. Qed.
 
 
     Section Relabeling_triple.
       Variable B' : Type.
 
-      Lemma relabeling_triple_preserves_is_in_ib (μ : B -> B') (t : @triple I B L) :
+      Lemma relabeling_triple_preserves_is_in_ib (μ : B -> B') (t : triple I B L) :
         is_in_ib (subject t) <-> is_in_ib (subject (relabeling_triple μ t)).
       Proof. case t => s /= _ _ _ _ _ /=. by apply relabeling_term_preserves_is_in_ib. Qed.
 
-      Lemma relabeling_triple_preserves_is_in_i (μ : B -> B') (t : @triple I B L) :
+      Lemma relabeling_triple_preserves_is_in_i (μ : B -> B') (t : triple I B L) :
         is_in_i (predicate t) <-> is_in_i (predicate (relabeling_triple μ t)).
       Proof. by case t => _ p /= _ _ _ _; apply relabeling_term_preserves_is_in_i. Qed.
 
-      Lemma relabeling_triple_preserves_is_in_ibl (μ : B -> B') (t : @triple I B L) :
+      Lemma relabeling_triple_preserves_is_in_ibl (μ : B -> B') (t : triple I B L) :
         is_in_ibl (object t) <-> is_in_ibl (object (relabeling_triple μ t)).
       Proof. by case t => _ _ o /= _ _ _; apply relabeling_term_preserves_is_in_ibl. Qed.
 
       Lemma relabeling_triple_ext (μ1 μ2 : B -> B') : μ1 =1 μ2 -> forall t, relabeling_triple μ1 t = relabeling_triple μ2 t.
-      Proof. move => μpweq t. apply /triple_inj; case t => /= [s p o _ _ _]; by apply (@relabeling_term_ext I B L B' μ1 μ2 μpweq). Qed.
+      Proof. move => μpweq t. apply /triple_inj; case t => /= [s p o _ _ _]; by apply (relabeling_term_ext μpweq). Qed.
 
     End Relabeling_triple.
   End PolyTriple.
@@ -69,7 +69,7 @@ Section Triple.
   Section EqTriple.
     Variable I B L : eqType.
 
-    Definition eqb_triple  (t1 t2 : @triple I B L) : bool :=
+    Definition eqb_triple  (t1 t2 : triple I B L) : bool :=
       ((subject t1) == (subject t2)) &&
         ((predicate t1) == (predicate t2)) &&
         ((object t1) == (object t2)).
@@ -83,13 +83,13 @@ Section Triple.
       by rewrite !eq_refl //.
     Qed.
 
-    Canonical triple_eqType := EqType triple (EqMixin triple_eqP).
+    Canonical triple_eqType := EqType (triple I B L) (EqMixin triple_eqP).
 
-    Definition terms_triple (t : @triple I B L) : seq term :=
+    Definition terms_triple (t : triple I B L) : seq (term I B L) :=
       let (s,p,o,_,_,_) := t in
       undup [:: s ; p ; o].
 
-    Definition bnodes_triple (t : @triple I B L) : seq (@term I B L) :=
+    Definition bnodes_triple (t : triple I B L) : seq (term I B L) :=
       undup (filter (@is_bnode I B L) (terms_triple t)).
 
   End EqTriple.
@@ -97,11 +97,11 @@ Section Triple.
   Section CountTriple.
     Variables I B L : countType.
 
-    Definition code_triple (t : @triple I B L) :=
+    Definition code_triple (t : triple I B L) :=
       let (s,p,o,_,_,_) := t in
       GenTree.Node 0 [:: (code_term s); (code_term p) ; (code_term o)].
 
-    Definition decode_triple (x : GenTree.tree nat) : option (@triple I B L).
+    Definition decode_triple (x : GenTree.tree nat) : option (triple I B L).
     Proof. destruct x eqn:E.
            - exact None.
            - destruct n as [| n'].
@@ -110,9 +110,9 @@ Section Triple.
                * exact None.
                * exact None.
                * destruct l0.
-                 -- destruct (@decode_term I B L s) as [dst | ] eqn:ds;
-                      destruct (@decode_term I B L p) as [dpt | ] eqn:dp;
-                      destruct (@decode_term I B L o) as [ dot| ] eqn:do.
+                 -- destruct (decode_term I B L s) as [dst | ] eqn:ds;
+                      destruct (decode_term I B L p) as [dpt | ] eqn:dp;
+                      destruct (decode_term I B L o) as [ dot| ] eqn:do.
                                                                         destruct (is_in_ib dst) eqn:iib;
                                                                           destruct (is_in_i dpt) eqn:ii;
                                                                           destruct (is_in_ibl dot) eqn: ibl.
@@ -123,7 +123,7 @@ Section Triple.
 
     Lemma cancel_triple_encode : pcancel code_triple decode_triple.
     Proof. case => s p o sib ii oibl. rewrite /code_triple /decode_triple.
-           have cant: forall (t : term), @decode_term I B L (code_term t) = Some t. apply cancel_code_decode.
+           have cant: forall (t : term I B L), decode_term I B L (code_term t) = Some t. apply cancel_code_decode.
            rewrite /= !cant; destruct s; destruct p ; destruct o => //=.
            all: by f_equal; apply triple_inj.
     Qed.
@@ -131,11 +131,11 @@ Section Triple.
     Definition triple_canChoiceMixin := PcanChoiceMixin cancel_triple_encode.
     Definition triple_canCountMixin := PcanCountMixin cancel_triple_encode.
 
-    Canonical triple_choiceType := Eval hnf in ChoiceType triple triple_canChoiceMixin.
-    Canonical triple_countType := Eval hnf in CountType triple triple_canCountMixin.
+    Canonical triple_choiceType := Eval hnf in ChoiceType (triple I B L) triple_canChoiceMixin.
+    Canonical triple_countType := Eval hnf in CountType (triple I B L) triple_canCountMixin.
 
     Definition triple_canPOrderMixin := PcanPOrderMixin (@pickleK triple_countType).
-    Canonical triple_POrderType := Eval hnf in POrderType tt triple triple_canPOrderMixin.
+    Canonical triple_POrderType := Eval hnf in POrderType tt (triple I B L) triple_canPOrderMixin.
 
   End CountTriple.
 End Triple.
